Test/tutorial/ImpVerifiedCompiler/ImpReductionContSem.dfy
@@ -34,7 +34,6 @@ predicate step(conf1: conf, conf2: conf) {
 			&& s2 == s1
 		case (CWhile(b, c), k) =>
 			&& (forall id: ident :: id_in_bexp(id,b) ==> id in s1)
-			&& !beval(s1, b)
 			&& c2 == (if beval(s1,b) then c else CSkip)
 			&& k2 == (if beval(s1,b) then Kwhile(b,c,k) else k1)
 			&& s2 == s1
